abp/SenderAutomaton.thy
@@ -3,14 +3,14 @@
  * This file was generated from Sender.maa and will be overridden when changed. To change
  * permanently, consider changing the model itself.
  *
- * Generated on Sep 18, 2018 2:23:42 PM by isartransformer 1.0.0
+ * Generated on Sep 19, 2018 11:04:38 PM by isartransformer 1.0.0
  *)
 theory SenderAutomaton
   imports bundle.tsynBundle automat.dAutomaton
 
 begin
 
-(* TODO Das sollte vielleicht wo anders hin *)
+(* Helper for easier generation *)
 fun prepend :: "'a::type list \<Rightarrow> 'a \<Rightarrow> 'a list" where
 "prepend xs x = x#xs"
 
@@ -36,6 +36,17 @@ end
 
 section \<open>Helpers to create a bundle from a single raw element\<close>
 
+(* Create one sbElem for all input streams *)
+fun createSbElem_As_I :: "(bool tsyn) \<Rightarrow> (nat tsyn) \<Rightarrow> (senderMessage tsyn sbElem)" where
+"createSbElem_As_I null null = Abs_sbElem [\<C> ''as'' \<mapsto> null, \<C> ''i'' \<mapsto> null]" |
+"createSbElem_As_I (Msg port_as) null = Abs_sbElem [\<C> ''as'' \<mapsto> Msg (SenderBool port_as), \<C> ''i'' \<mapsto> null]" |
+"createSbElem_As_I null (Msg port_i) = Abs_sbElem [\<C> ''as'' \<mapsto> null, \<C> ''i'' \<mapsto> Msg (SenderNat port_i)]" |
+"createSbElem_As_I (Msg port_as) (Msg port_i) = Abs_sbElem [\<C> ''as'' \<mapsto> Msg (SenderBool port_as), \<C> ''i'' \<mapsto> Msg (SenderNat port_i)]"
+
+(* Create one SB for all input streams *)
+fun createBundle_As_I :: "(bool tsyn) \<Rightarrow> (nat tsyn) \<Rightarrow> (senderMessage tsyn SB)" where
+"createBundle_As_I port_as  port_i  = (sbe2SB (createSbElem_As_I port_as  port_i ))"
+
 lift_definition createAsBundle :: "bool \<Rightarrow> senderMessage tsyn sbElem" is
 "\<lambda>x. [\<C> ''as'' \<mapsto> Msg (SenderBool x)]"
   unfolding sbElemWell_def
@@ -60,31 +71,37 @@ lift_definition createDsBundle :: "(nat\<times>bool) \<Rightarrow> senderMessage
 
 section \<open>Helpers to create a bundle from a single tsyn element\<close>
 
-fun createTsynAsBundle :: "bool tsyn \<Rightarrow> senderMessage tsyn sbElem" where
-"createTsynAsBundle (Msg x) = (createAsBundle x)" |
-"createTsynAsBundle null = (sbeNull {\<C> ''as''})"
+fun createTsynAsBundle :: "bool tsyn \<Rightarrow> senderMessage tsyn SB" where
+"createTsynAsBundle (Msg x) = sbe2SB (createAsBundle x)" |
+"createTsynAsBundle null = sbe2SB (sbeNull {\<C> ''as''})"
 
-fun createTsynIBundle :: "nat tsyn \<Rightarrow> senderMessage tsyn sbElem" where
-"createTsynIBundle (Msg x) = (createIBundle x)" |
-"createTsynIBundle null = (sbeNull {\<C> ''i''})"
+declare createTsynAsBundle.simps[simp del]
 
-fun createTsynDsBundle :: "(nat\<times>bool) tsyn \<Rightarrow> senderMessage tsyn sbElem" where
-"createTsynDsBundle (Msg x) = (createDsBundle x)" |
-"createTsynDsBundle null = (sbeNull {\<C> ''ds''})"
+fun createTsynIBundle :: "nat tsyn \<Rightarrow> senderMessage tsyn SB" where
+"createTsynIBundle (Msg x) = sbe2SB (createIBundle x)" |
+"createTsynIBundle null = sbe2SB (sbeNull {\<C> ''i''})"
+
+declare createTsynIBundle.simps[simp del]
+
+fun createTsynDsBundle :: "(nat\<times>bool) tsyn \<Rightarrow> senderMessage tsyn SB" where
+"createTsynDsBundle (Msg x) = sbe2SB (createDsBundle x)" |
+"createTsynDsBundle null = sbe2SB (sbeNull {\<C> ''ds''})"
+
+declare createTsynDsBundle.simps[simp del]
 
 
 section \<open>Helpers to create a bundle from a tsyn list of elements\<close>
 
 fun createLongAsBundle :: "(bool tsyn) list \<Rightarrow> senderMessage tsyn SB" where
-"createLongAsBundle (x#xs) = ubConcEq (sbe2SB (createTsynAsBundle x))\<cdot>(createLongAsBundle xs)" |
+"createLongAsBundle (x#xs) = ubConcEq (createTsynAsBundle x)\<cdot>(createLongAsBundle xs)" |
 "createLongAsBundle []     = ubLeast {\<C> ''as''}"
 
 fun createLongIBundle :: "(nat tsyn) list \<Rightarrow> senderMessage tsyn SB" where
-"createLongIBundle (x#xs) = ubConcEq (sbe2SB (createTsynIBundle x))\<cdot>(createLongIBundle xs)" |
+"createLongIBundle (x#xs) = ubConcEq (createTsynIBundle x)\<cdot>(createLongIBundle xs)" |
 "createLongIBundle []     = ubLeast {\<C> ''i''}"
 
 fun createLongDsBundle :: "((nat\<times>bool) tsyn) list \<Rightarrow> senderMessage tsyn SB" where
-"createLongDsBundle (x#xs) = ubConcEq (sbe2SB (createTsynDsBundle x))\<cdot>(createLongDsBundle xs)" |
+"createLongDsBundle (x#xs) = ubConcEq (createTsynDsBundle x)\<cdot>(createLongDsBundle xs)" |
 "createLongDsBundle []     = ubLeast {\<C> ''ds''}"
 
 
@@ -129,22 +146,22 @@ lemma createDsBundle_len [simp]: "ubLen (sbe2SB (createDsBundle x)) = Fin 1"
 
 section \<open>Lemmas for "createTsynXBundle"\<close>
 
-lemma createTsynAsBundle_dom [simp]: "sbeDom (createTsynAsBundle x) = {\<C> ''as''}"
-  by (cases x, simp_all)
+lemma createTsynAsBundle_dom [simp]: "ubDom\<cdot>(createTsynAsBundle x) = {\<C> ''as''}"
+  by (cases x, simp_all add: createTsynAsBundle.simps)
 
 lemma createTsynAsBundle_len [simp]: "ubLen (sbe2DB (createTsynAsBundle x)) = Fin 1"
   apply (cases x, simp_all)
   oops
 
-lemma createTsynIBundle_dom [simp]: "sbeDom (createTsynIBundle x) = {\<C> ''i''}"
-  by (cases x, simp_all)
+lemma createTsynIBundle_dom [simp]: "ubDom\<cdot>(createTsynIBundle x) = {\<C> ''i''}"
+  by (cases x, simp_all add: createTsynIBundle.simps)
 
 lemma createTsynIBundle_len [simp]: "ubLen (sbe2DB (createTsynIBundle x)) = Fin 1"
   apply (cases x, simp_all)
   oops
 
-lemma createTsynDsBundle_dom [simp]: "sbeDom (createTsynDsBundle x) = {\<C> ''ds''}"
-  by (cases x, simp_all)
+lemma createTsynDsBundle_dom [simp]: "ubDom\<cdot>(createTsynDsBundle x) = {\<C> ''ds''}"
+  by (cases x, simp_all add: createTsynDsBundle.simps)
 
 lemma createTsynDsBundle_len [simp]: "ubLen (sbe2DB (createTsynDsBundle x)) = Fin 1"
   apply (cases x, simp_all)
@@ -284,237 +301,470 @@ fun senderTransitionH :: "(SenderState \<times> (senderMessage tsyn \<times> sen
 fun senderTransition :: "(SenderState \<times> senderMessage tsyn sbElem) \<Rightarrow> (SenderState \<times> senderMessage tsyn SB)" where
 "senderTransition (s,b) = (if (sbeDom b) = {\<C> ''as'', \<C> ''i''} then senderTransitionH (s, (Rep_sbElem b\<rightharpoonup>\<C> ''as'', Rep_sbElem b\<rightharpoonup>\<C> ''i'')) else undefined)"
 
+(* The final automaton *)
 lift_definition SenderAutomaton :: "(SenderState, senderMessage tsyn) dAutomaton" is
 "(senderTransition, SenderState St []  0, tsynbNull (\<C> ''ds''), {\<C> ''as'', \<C> ''i''}, {\<C> ''ds''})"
   by simp
 
+(* Stream processing function for each state (handy for step lemmata) *)
+definition SenderStep :: "(SenderState \<Rightarrow> (senderMessage tsyn, senderMessage tsyn) SPF)" where
+"SenderStep = da_h SenderAutomaton"
+
+(* The final SPF *)
 definition SenderSPF :: "(senderMessage tsyn, senderMessage tsyn) SPF" where
 "SenderSPF = da_H SenderAutomaton"
 
 
-section \<open>Lemmata for the transitions\<close>
+section \<open>Step-wise lemmata for the transition function\<close>
 
-(* Line 33 in the MAA model *)
-lemma tbd_0_0:
+(* Line 33:  Sf -> St [buffer.size()>1 && i!=null] {as==false} / {buffer=buffer.butlast().prepend(i), c=3, ds=new Pair<>(buffer.butlast().last(),true)}; *)
+lemma transition_0_0:
   assumes "(size var_buffer)>1 \<and> port_as=False"
-    shows "spfConcIn  (sbe2DB (createAsBundle port_as) \<uplus> sbe2SB (createIBundle port_i))\<cdot>(da_h SenderAutomaton (SenderState Sf var_buffer var_c))
+    shows "senderTransition ((SenderState Sf var_buffer var_c), (createSbElem_As_I (Msg port_as) (Msg port_i)))
+         = (SenderState St (prepend (butlast var_buffer) port_i) 3, (sbe2SB (createDsBundle (Pair (last (butlast var_buffer)) True))))"
+  oops
+
+(* Line 35:  Sf -> St [buffer.size()=1 && i!=null] {as==false} / {buffer=buffer.butlast().prepend(i), c=3, ds=new Pair<>(i,true)}; *)
+lemma transition_0_1:
+  assumes "(size var_buffer)=1 \<and> port_as=False"
+    shows "senderTransition ((SenderState Sf var_buffer var_c), (createSbElem_As_I (Msg port_as) (Msg port_i)))
+         = (SenderState St (prepend (butlast var_buffer) port_i) 3, (sbe2SB (createDsBundle (Pair port_i True))))"
+  oops
+
+(* Line 43:  Sf -> Sf [buffer.size()=0 && as!=null && i!=null] / {buffer=buffer.prepend(i), c=3, ds=new Pair<>(i,false)}; *)
+lemma transition_0_2:
+  assumes "(size var_buffer)=0"
+    shows "senderTransition ((SenderState Sf var_buffer var_c), (createSbElem_As_I (Msg port_as) (Msg port_i)))
+         = (SenderState Sf (prepend var_buffer port_i) 3, (sbe2SB (createDsBundle (Pair port_i False))))"
+  oops
+
+(* Line 45:  Sf -> Sf [buffer.size()>0 && c>0 && i!=null] {as==true} / {buffer=buffer.prepend(i), c=c-1}; *)
+lemma transition_0_3:
+  assumes "(size var_buffer)>0 \<and> var_c>0 \<and> port_as=True"
+    shows "senderTransition ((SenderState Sf var_buffer var_c), (createSbElem_As_I (Msg port_as) (Msg port_i)))
+         = (SenderState Sf (prepend var_buffer port_i) (var_c-1), (tsynbNull (\<C> ''ds'')))"
+  oops
+
+(* Line 47:  Sf -> Sf [buffer.size()>0 && c=0 && i!=null] {as==true} / {buffer=buffer.prepend(i), c=3, ds=new Pair<>(buffer.last(),false)}; *)
+lemma transition_0_4:
+  assumes "(size var_buffer)>0 \<and> var_c=0 \<and> port_as=True"
+    shows "senderTransition ((SenderState Sf var_buffer var_c), (createSbElem_As_I (Msg port_as) (Msg port_i)))
+         = (SenderState Sf (prepend var_buffer port_i) 3, (sbe2SB (createDsBundle (Pair (last var_buffer) False))))"
+  oops
+
+(* Line 34:  Sf -> St [buffer.size()>1] {as==false, i==null} / {buffer=buffer.butlast(), c=3, ds=new Pair<>(buffer.butlast().last(),true)}; *)
+lemma transition_1_0:
+  assumes "(size var_buffer)>1 \<and> port_as=False"
+    shows "senderTransition ((SenderState Sf var_buffer var_c), (createSbElem_As_I (Msg port_as) null))
+         = (SenderState St (butlast var_buffer) 3, (sbe2SB (createDsBundle (Pair (last (butlast var_buffer)) True))))"
+  oops
+
+(* Line 36:  Sf -> St [buffer.size()=1] {as==false, i==null} / {buffer=buffer.butlast()}; *)
+lemma transition_1_1:
+  assumes "(size var_buffer)=1 \<and> port_as=False"
+    shows "senderTransition ((SenderState Sf var_buffer var_c), (createSbElem_As_I (Msg port_as) null))
+         = (SenderState St (butlast var_buffer) var_c, (tsynbNull (\<C> ''ds'')))"
+  oops
+
+(* Line 38:  Sf -> Sf [buffer.size()=0 && as!=null] {i==null}; *)
+lemma transition_1_2:
+  assumes "(size var_buffer)=0"
+    shows "senderTransition ((SenderState Sf var_buffer var_c), (createSbElem_As_I (Msg port_as) null))
+         = (SenderState Sf var_buffer var_c, (tsynbNull (\<C> ''ds'')))"
+  oops
+
+(* Line 40:  Sf -> Sf [buffer.size()>0 && c>0] {as==true, i==null} / {c=c-1}; *)
+lemma transition_1_3:
+  assumes "(size var_buffer)>0 \<and> var_c>0 \<and> port_as=True"
+    shows "senderTransition ((SenderState Sf var_buffer var_c), (createSbElem_As_I (Msg port_as) null))
+         = (SenderState Sf var_buffer (var_c-1), (tsynbNull (\<C> ''ds'')))"
+  oops
+
+(* Line 41:  Sf -> Sf [buffer.size()>0 && c=0] {as==true, i==null} / {c=3, ds=new Pair<>(buffer.last(),false)}; *)
+lemma transition_1_4:
+  assumes "(size var_buffer)>0 \<and> var_c=0 \<and> port_as=True"
+    shows "senderTransition ((SenderState Sf var_buffer var_c), (createSbElem_As_I (Msg port_as) null))
+         = (SenderState Sf var_buffer 3, (sbe2SB (createDsBundle (Pair (last var_buffer) False))))"
+  oops
+
+(* Line 44:  Sf -> Sf [buffer.size()=0 && i!=null] {as==null} / {buffer=buffer.prepend(i), c=3, ds=new Pair<>(i,false)}; *)
+lemma transition_2_0:
+  assumes "(size var_buffer)=0"
+    shows "senderTransition ((SenderState Sf var_buffer var_c), (createSbElem_As_I null (Msg port_i)))
+         = (SenderState Sf (prepend var_buffer port_i) 3, (sbe2SB (createDsBundle (Pair port_i False))))"
+  oops
+
+(* Line 46:  Sf -> Sf [buffer.size()>0 && c>0 && i!=null] {as==null} / {buffer=buffer.prepend(i), c=c-1}; *)
+lemma transition_2_1:
+  assumes "(size var_buffer)>0 \<and> var_c>0"
+    shows "senderTransition ((SenderState Sf var_buffer var_c), (createSbElem_As_I null (Msg port_i)))
+         = (SenderState Sf (prepend var_buffer port_i) (var_c-1), (tsynbNull (\<C> ''ds'')))"
+  oops
+
+(* Line 48:  Sf -> Sf [buffer.size()>0 && c=0 && i!=null] {as==null} / {buffer=buffer.prepend(i), c=3, ds=new Pair<>(buffer.last(),false)}; *)
+lemma transition_2_2:
+  assumes "(size var_buffer)>0 \<and> var_c=0"
+    shows "senderTransition ((SenderState Sf var_buffer var_c), (createSbElem_As_I null (Msg port_i)))
+         = (SenderState Sf (prepend var_buffer port_i) 3, (sbe2SB (createDsBundle (Pair (last var_buffer) False))))"
+  oops
+
+(* Line 37:  Sf -> Sf [buffer.size()=0] {as==null, i==null}; *)
+lemma transition_3_0:
+  assumes "(size var_buffer)=0"
+    shows "senderTransition ((SenderState Sf var_buffer var_c), (createSbElem_As_I null null))
+         = (SenderState Sf var_buffer var_c, (tsynbNull (\<C> ''ds'')))"
+  oops
+
+(* Line 39:  Sf -> Sf [buffer.size()>0 && c>0] {as==null, i==null}; *)
+lemma transition_3_1:
+  assumes "(size var_buffer)>0 \<and> var_c>0"
+    shows "senderTransition ((SenderState Sf var_buffer var_c), (createSbElem_As_I null null))
+         = (SenderState Sf var_buffer var_c, (tsynbNull (\<C> ''ds'')))"
+  oops
+
+(* Line 42:  Sf -> Sf [buffer.size()>0 && c=0] {as==null, i==null} / {c=3, ds=new Pair<>(buffer.last(),false)}; *)
+lemma transition_3_2:
+  assumes "(size var_buffer)>0 \<and> var_c=0"
+    shows "senderTransition ((SenderState Sf var_buffer var_c), (createSbElem_As_I null null))
+         = (SenderState Sf var_buffer 3, (sbe2SB (createDsBundle (Pair (last var_buffer) False))))"
+  oops
+
+(* Line 25:  St -> St [buffer.size()=0 && as!=null && i!=null] / {buffer=buffer.prepend(i), c=3, ds=new Pair<>(i,true)}; *)
+lemma transition_4_0:
+  assumes "(size var_buffer)=0"
+    shows "senderTransition ((SenderState St var_buffer var_c), (createSbElem_As_I (Msg port_as) (Msg port_i)))
+         = (SenderState St (prepend var_buffer port_i) 3, (sbe2SB (createDsBundle (Pair port_i True))))"
+  oops
+
+(* Line 27:  St -> Sf [buffer.size()>1 && i!=null] {as==true} / {buffer=buffer.butlast().prepend(i), c=3, ds=new Pair<>(buffer.butlast().last(),false)}; *)
+lemma transition_4_1:
+  assumes "(size var_buffer)>1 \<and> port_as=True"
+    shows "senderTransition ((SenderState St var_buffer var_c), (createSbElem_As_I (Msg port_as) (Msg port_i)))
+         = (SenderState Sf (prepend (butlast var_buffer) port_i) 3, (sbe2SB (createDsBundle (Pair (last (butlast var_buffer)) False))))"
+  oops
+
+(* Line 28:  St -> St [buffer.size()>0 && c>0 && i!=null] {as==false} / {buffer=buffer.prepend(i), c=c-1}; *)
+lemma transition_4_2:
+  assumes "(size var_buffer)>0 \<and> var_c>0 \<and> port_as=False"
+    shows "senderTransition ((SenderState St var_buffer var_c), (createSbElem_As_I (Msg port_as) (Msg port_i)))
+         = (SenderState St (prepend var_buffer port_i) (var_c-1), (tsynbNull (\<C> ''ds'')))"
+  oops
+
+(* Line 30:  St -> St [buffer.size()>0 && c=0 && i!=null] {as==false} / {buffer=buffer.prepend(i), c=3, ds=new Pair<>(buffer.last(),true)}; *)
+lemma transition_4_3:
+  assumes "(size var_buffer)>0 \<and> var_c=0 \<and> port_as=False"
+    shows "senderTransition ((SenderState St var_buffer var_c), (createSbElem_As_I (Msg port_as) (Msg port_i)))
+         = (SenderState St (prepend var_buffer port_i) 3, (sbe2SB (createDsBundle (Pair (last var_buffer) True))))"
+  oops
+
+(* Line 32:  St -> Sf [buffer.size()=1 && i!=null] {as==true} / {buffer=buffer.butlast().prepend(i), c=3, ds=new Pair<>(i,false)}; *)
+lemma transition_4_4:
+  assumes "(size var_buffer)=1 \<and> port_as=True"
+    shows "senderTransition ((SenderState St var_buffer var_c), (createSbElem_As_I (Msg port_as) (Msg port_i)))
+         = (SenderState Sf (prepend (butlast var_buffer) port_i) 3, (sbe2SB (createDsBundle (Pair port_i False))))"
+  oops
+
+(* Line 17:  St -> St [buffer.size()=0 && as!=null] {i==null}; *)
+lemma transition_5_0:
+  assumes "(size var_buffer)=0"
+    shows "senderTransition ((SenderState St var_buffer var_c), (createSbElem_As_I (Msg port_as) null))
+         = (SenderState St var_buffer var_c, (tsynbNull (\<C> ''ds'')))"
+  oops
+
+(* Line 18:  St -> Sf [buffer.size()>1] {as==true, i==null} / {buffer=buffer.butlast(), c=3, ds=new Pair<>(buffer.butlast().last(),false)}; *)
+lemma transition_5_1:
+  assumes "(size var_buffer)>1 \<and> port_as=True"
+    shows "senderTransition ((SenderState St var_buffer var_c), (createSbElem_As_I (Msg port_as) null))
+         = (SenderState Sf (butlast var_buffer) 3, (sbe2SB (createDsBundle (Pair (last (butlast var_buffer)) False))))"
+  oops
+
+(* Line 20:  St -> St [buffer.size()>0 && c>0] {as==false, i==null} / {c=c-1}; *)
+lemma transition_5_2:
+  assumes "(size var_buffer)>0 \<and> var_c>0 \<and> port_as=False"
+    shows "senderTransition ((SenderState St var_buffer var_c), (createSbElem_As_I (Msg port_as) null))
+         = (SenderState St var_buffer (var_c-1), (tsynbNull (\<C> ''ds'')))"
+  oops
+
+(* Line 22:  St -> St [buffer.size()>0 && c=0] {as==false, i==null} / {c=3, ds=new Pair<>(buffer.last(),true)}; *)
+lemma transition_5_3:
+  assumes "(size var_buffer)>0 \<and> var_c=0 \<and> port_as=False"
+    shows "senderTransition ((SenderState St var_buffer var_c), (createSbElem_As_I (Msg port_as) null))
+         = (SenderState St var_buffer 3, (sbe2SB (createDsBundle (Pair (last var_buffer) True))))"
+  oops
+
+(* Line 24:  St -> Sf [buffer.size()=1] {as==true, i==null} / {buffer=buffer.butlast()}; *)
+lemma transition_5_4:
+  assumes "(size var_buffer)=1 \<and> port_as=True"
+    shows "senderTransition ((SenderState St var_buffer var_c), (createSbElem_As_I (Msg port_as) null))
+         = (SenderState Sf (butlast var_buffer) var_c, (tsynbNull (\<C> ''ds'')))"
+  oops
+
+(* Line 26:  St -> St [buffer.size()=0 && i!=null] {as==null} / {buffer=buffer.prepend(i), c=3, ds=new Pair<>(i,true)}; *)
+lemma transition_6_0:
+  assumes "(size var_buffer)=0"
+    shows "senderTransition ((SenderState St var_buffer var_c), (createSbElem_As_I null (Msg port_i)))
+         = (SenderState St (prepend var_buffer port_i) 3, (sbe2SB (createDsBundle (Pair port_i True))))"
+  oops
+
+(* Line 29:  St -> St [buffer.size()>0 && c>0 && i!=null] {as==null} / {buffer=buffer.prepend(i), c=c-1}; *)
+lemma transition_6_1:
+  assumes "(size var_buffer)>0 \<and> var_c>0"
+    shows "senderTransition ((SenderState St var_buffer var_c), (createSbElem_As_I null (Msg port_i)))
+         = (SenderState St (prepend var_buffer port_i) (var_c-1), (tsynbNull (\<C> ''ds'')))"
+  oops
+
+(* Line 31:  St -> St [buffer.size()>0 && c=0 && i!=null] {as==null} / {buffer=buffer.prepend(i), c=3, ds=new Pair<>(buffer.last(),true)}; *)
+lemma transition_6_2:
+  assumes "(size var_buffer)>0 \<and> var_c=0"
+    shows "senderTransition ((SenderState St var_buffer var_c), (createSbElem_As_I null (Msg port_i)))
+         = (SenderState St (prepend var_buffer port_i) 3, (sbe2SB (createDsBundle (Pair (last var_buffer) True))))"
+  oops
+
+(* Line 19:  St -> St [buffer.size()=0] {as==null, i==null}; *)
+lemma transition_7_0:
+  assumes "(size var_buffer)=0"
+    shows "senderTransition ((SenderState St var_buffer var_c), (createSbElem_As_I null null))
+         = (SenderState St var_buffer var_c, (tsynbNull (\<C> ''ds'')))"
+  oops
+
+(* Line 21:  St -> St [buffer.size()>0 && c>0] {as==null, i==null} / {c=c-1}; *)
+lemma transition_7_1:
+  assumes "(size var_buffer)>0 \<and> var_c>0"
+    shows "senderTransition ((SenderState St var_buffer var_c), (createSbElem_As_I null null))
+         = (SenderState St var_buffer (var_c-1), (tsynbNull (\<C> ''ds'')))"
+  oops
+
+(* Line 23:  St -> St [buffer.size()>0 && c=0] {as==null, i==null} / {c=3, ds=new Pair<>(buffer.last(),true)}; *)
+lemma transition_7_2:
+  assumes "(size var_buffer)>0 \<and> var_c=0"
+    shows "senderTransition ((SenderState St var_buffer var_c), (createSbElem_As_I null null))
+         = (SenderState St var_buffer 3, (sbe2SB (createDsBundle (Pair (last var_buffer) True))))"
+  oops
+
+
+section \<open>Step-wise lemmata for the SPF\<close>
+
+(* Line 33:  Sf -> St [buffer.size()>1 && i!=null] {as==false} / {buffer=buffer.butlast().prepend(i), c=3, ds=new Pair<>(buffer.butlast().last(),true)}; *)
+lemma step_0_0:
+  assumes "(size var_buffer)>1 \<and> port_as=False"
+    shows "spfConcIn  (createBundle_As_I (Msg port_as) (Msg port_i))\<cdot>(da_h SenderAutomaton (SenderState Sf var_buffer var_c))
          = spfConcOut (sbe2SB (createDsBundle (Pair (last (butlast var_buffer)) True)))\<cdot>(da_h SenderAutomaton (SenderState St (prepend (butlast var_buffer) port_i) 3))"
   oops
 
-(* Line 35 in the MAA model *)
-lemma tbd_0_1:
+(* Line 35:  Sf -> St [buffer.size()=1 && i!=null] {as==false} / {buffer=buffer.butlast().prepend(i), c=3, ds=new Pair<>(i,true)}; *)
+lemma step_0_1:
   assumes "(size var_buffer)=1 \<and> port_as=False"
-    shows "spfConcIn  (sbe2DB (createAsBundle port_as) \<uplus> sbe2SB (createIBundle port_i))\<cdot>(da_h SenderAutomaton (SenderState Sf var_buffer var_c))
+    shows "spfConcIn  (createBundle_As_I (Msg port_as) (Msg port_i))\<cdot>(da_h SenderAutomaton (SenderState Sf var_buffer var_c))
          = spfConcOut (sbe2SB (createDsBundle (Pair port_i True)))\<cdot>(da_h SenderAutomaton (SenderState St (prepend (butlast var_buffer) port_i) 3))"
   oops
 
-(* Line 43 in the MAA model *)
-lemma tbd_0_2:
+(* Line 43:  Sf -> Sf [buffer.size()=0 && as!=null && i!=null] / {buffer=buffer.prepend(i), c=3, ds=new Pair<>(i,false)}; *)
+lemma step_0_2:
   assumes "(size var_buffer)=0"
-    shows "spfConcIn  (sbe2SB (createAsBundle port_as) \<uplus> sbe2SB (createIBundle port_i))\<cdot>(da_h SenderAutomaton (SenderState Sf var_buffer var_c))
+    shows "spfConcIn  (createBundle_As_I (Msg port_as) (Msg port_i))\<cdot>(da_h SenderAutomaton (SenderState Sf var_buffer var_c))
          = spfConcOut (sbe2SB (createDsBundle (Pair port_i False)))\<cdot>(da_h SenderAutomaton (SenderState Sf (prepend var_buffer port_i) 3))"
   oops
 
-(* Line 45 in the MAA model *)
-lemma tbd_0_3:
+(* Line 45:  Sf -> Sf [buffer.size()>0 && c>0 && i!=null] {as==true} / {buffer=buffer.prepend(i), c=c-1}; *)
+lemma step_0_3:
   assumes "(size var_buffer)>0 \<and> var_c>0 \<and> port_as=True"
-    shows "spfConcIn  (sbe2DB (createAsBundle port_as) \<uplus> sbe2SB (createIBundle port_i))\<cdot>(da_h SenderAutomaton (SenderState Sf var_buffer var_c))
+    shows "spfConcIn  (createBundle_As_I (Msg port_as) (Msg port_i))\<cdot>(da_h SenderAutomaton (SenderState Sf var_buffer var_c))
          = spfConcOut (tsynbNull (\<C> ''ds''))\<cdot>(da_h SenderAutomaton (SenderState Sf (prepend var_buffer port_i) (var_c-1)))"
   oops
 
-(* Line 47 in the MAA model *)
-lemma tbd_0_4:
+(* Line 47:  Sf -> Sf [buffer.size()>0 && c=0 && i!=null] {as==true} / {buffer=buffer.prepend(i), c=3, ds=new Pair<>(buffer.last(),false)}; *)
+lemma step_0_4:
   assumes "(size var_buffer)>0 \<and> var_c=0 \<and> port_as=True"
-    shows "spfConcIn  (sbe2DB (createAsBundle port_as) \<uplus> sbe2SB (createIBundle port_i))\<cdot>(da_h SenderAutomaton (SenderState Sf var_buffer var_c))
+    shows "spfConcIn  (createBundle_As_I (Msg port_as) (Msg port_i))\<cdot>(da_h SenderAutomaton (SenderState Sf var_buffer var_c))
          = spfConcOut (sbe2SB (createDsBundle (Pair (last var_buffer) False)))\<cdot>(da_h SenderAutomaton (SenderState Sf (prepend var_buffer port_i) 3))"
   oops
 
-(* Line 34 in the MAA model *)
-lemma tbd_1_0:
+(* Line 34:  Sf -> St [buffer.size()>1] {as==false, i==null} / {buffer=buffer.butlast(), c=3, ds=new Pair<>(buffer.butlast().last(),true)}; *)
+lemma step_1_0:
   assumes "(size var_buffer)>1 \<and> port_as=False"
-    shows "spfConcIn  (sbe2DB (createAsBundle port_as) \<uplus> tsynbNull (\<C> ''i''))\<cdot>(da_h SenderAutomaton (SenderState Sf var_buffer var_c))
+    shows "spfConcIn  (createBundle_As_I (Msg port_as) null)\<cdot>(da_h SenderAutomaton (SenderState Sf var_buffer var_c))
          = spfConcOut (sbe2SB (createDsBundle (Pair (last (butlast var_buffer)) True)))\<cdot>(da_h SenderAutomaton (SenderState St (butlast var_buffer) 3))"
   oops
 
-(* Line 36 in the MAA model *)
-lemma tbd_1_1:
+(* Line 36:  Sf -> St [buffer.size()=1] {as==false, i==null} / {buffer=buffer.butlast()}; *)
+lemma step_1_1:
   assumes "(size var_buffer)=1 \<and> port_as=False"
-    shows "spfConcIn  (sbe2DB (createAsBundle port_as) \<uplus> tsynbNull (\<C> ''i''))\<cdot>(da_h SenderAutomaton (SenderState Sf var_buffer var_c))
+    shows "spfConcIn  (createBundle_As_I (Msg port_as) null)\<cdot>(da_h SenderAutomaton (SenderState Sf var_buffer var_c))
          = spfConcOut (tsynbNull (\<C> ''ds''))\<cdot>(da_h SenderAutomaton (SenderState St (butlast var_buffer) var_c))"
   oops
 
-(* Line 38 in the MAA model *)
-lemma tbd_1_2:
+(* Line 38:  Sf -> Sf [buffer.size()=0 && as!=null] {i==null}; *)
+lemma step_1_2:
   assumes "(size var_buffer)=0"
-    shows "spfConcIn  (sbe2SB (createAsBundle port_as) \<uplus> tsynbNull (\<C> ''i''))\<cdot>(da_h SenderAutomaton (SenderState Sf var_buffer var_c))
+    shows "spfConcIn  (createBundle_As_I (Msg port_as) null)\<cdot>(da_h SenderAutomaton (SenderState Sf var_buffer var_c))
          = spfConcOut (tsynbNull (\<C> ''ds''))\<cdot>(da_h SenderAutomaton (SenderState Sf var_buffer var_c))"
   oops
 
-(* Line 40 in the MAA model *)
-lemma tbd_1_3:
+(* Line 40:  Sf -> Sf [buffer.size()>0 && c>0] {as==true, i==null} / {c=c-1}; *)
+lemma step_1_3:
   assumes "(size var_buffer)>0 \<and> var_c>0 \<and> port_as=True"
-    shows "spfConcIn  (sbe2DB (createAsBundle port_as) \<uplus> tsynbNull (\<C> ''i''))\<cdot>(da_h SenderAutomaton (SenderState Sf var_buffer var_c))
+    shows "spfConcIn  (createBundle_As_I (Msg port_as) null)\<cdot>(da_h SenderAutomaton (SenderState Sf var_buffer var_c))
          = spfConcOut (tsynbNull (\<C> ''ds''))\<cdot>(da_h SenderAutomaton (SenderState Sf var_buffer (var_c-1)))"
   oops
 
-(* Line 41 in the MAA model *)
-lemma tbd_1_4:
+(* Line 41:  Sf -> Sf [buffer.size()>0 && c=0] {as==true, i==null} / {c=3, ds=new Pair<>(buffer.last(),false)}; *)
+lemma step_1_4:
   assumes "(size var_buffer)>0 \<and> var_c=0 \<and> port_as=True"
-    shows "spfConcIn  (sbe2DB (createAsBundle port_as) \<uplus> tsynbNull (\<C> ''i''))\<cdot>(da_h SenderAutomaton (SenderState Sf var_buffer var_c))
+    shows "spfConcIn  (createBundle_As_I (Msg port_as) null)\<cdot>(da_h SenderAutomaton (SenderState Sf var_buffer var_c))
          = spfConcOut (sbe2SB (createDsBundle (Pair (last var_buffer) False)))\<cdot>(da_h SenderAutomaton (SenderState Sf var_buffer 3))"
   oops
 
-(* Line 44 in the MAA model *)
-lemma tbd_2_0:
+(* Line 44:  Sf -> Sf [buffer.size()=0 && i!=null] {as==null} / {buffer=buffer.prepend(i), c=3, ds=new Pair<>(i,false)}; *)
+lemma step_2_0:
   assumes "(size var_buffer)=0"
-    shows "spfConcIn  (tsynbNull (\<C> ''as'') \<uplus> sbe2SB (createIBundle port_i))\<cdot>(da_h SenderAutomaton (SenderState Sf var_buffer var_c))
+    shows "spfConcIn  (createBundle_As_I null (Msg port_i))\<cdot>(da_h SenderAutomaton (SenderState Sf var_buffer var_c))
          = spfConcOut (sbe2SB (createDsBundle (Pair port_i False)))\<cdot>(da_h SenderAutomaton (SenderState Sf (prepend var_buffer port_i) 3))"
   oops
 
-(* Line 46 in the MAA model *)
-lemma tbd_2_1:
+(* Line 46:  Sf -> Sf [buffer.size()>0 && c>0 && i!=null] {as==null} / {buffer=buffer.prepend(i), c=c-1}; *)
+lemma step_2_1:
   assumes "(size var_buffer)>0 \<and> var_c>0"
-    shows "spfConcIn  (tsynbNull (\<C> ''as'') \<uplus> sbe2SB (createIBundle port_i))\<cdot>(da_h SenderAutomaton (SenderState Sf var_buffer var_c))
+    shows "spfConcIn  (createBundle_As_I null (Msg port_i))\<cdot>(da_h SenderAutomaton (SenderState Sf var_buffer var_c))
          = spfConcOut (tsynbNull (\<C> ''ds''))\<cdot>(da_h SenderAutomaton (SenderState Sf (prepend var_buffer port_i) (var_c-1)))"
   oops
 
-(* Line 48 in the MAA model *)
-lemma tbd_2_2:
+(* Line 48:  Sf -> Sf [buffer.size()>0 && c=0 && i!=null] {as==null} / {buffer=buffer.prepend(i), c=3, ds=new Pair<>(buffer.last(),false)}; *)
+lemma step_2_2:
   assumes "(size var_buffer)>0 \<and> var_c=0"
-    shows "spfConcIn  (tsynbNull (\<C> ''as'') \<uplus> sbe2SB (createIBundle port_i))\<cdot>(da_h SenderAutomaton (SenderState Sf var_buffer var_c))
+    shows "spfConcIn  (createBundle_As_I null (Msg port_i))\<cdot>(da_h SenderAutomaton (SenderState Sf var_buffer var_c))
          = spfConcOut (sbe2SB (createDsBundle (Pair (last var_buffer) False)))\<cdot>(da_h SenderAutomaton (SenderState Sf (prepend var_buffer port_i) 3))"
   oops
 
-(* Line 37 in the MAA model *)
-lemma tbd_3_0:
+(* Line 37:  Sf -> Sf [buffer.size()=0] {as==null, i==null}; *)
+lemma step_3_0:
   assumes "(size var_buffer)=0"
-    shows "spfConcIn  (tsynbNull (\<C> ''as'') \<uplus> tsynbNull (\<C> ''i''))\<cdot>(da_h SenderAutomaton (SenderState Sf var_buffer var_c))
+    shows "spfConcIn  (createBundle_As_I null null)\<cdot>(da_h SenderAutomaton (SenderState Sf var_buffer var_c))
          = spfConcOut (tsynbNull (\<C> ''ds''))\<cdot>(da_h SenderAutomaton (SenderState Sf var_buffer var_c))"
   oops
 
-(* Line 39 in the MAA model *)
-lemma tbd_3_1:
+(* Line 39:  Sf -> Sf [buffer.size()>0 && c>0] {as==null, i==null}; *)
+lemma step_3_1:
   assumes "(size var_buffer)>0 \<and> var_c>0"
-    shows "spfConcIn  (tsynbNull (\<C> ''as'') \<uplus> tsynbNull (\<C> ''i''))\<cdot>(da_h SenderAutomaton (SenderState Sf var_buffer var_c))
+    shows "spfConcIn  (createBundle_As_I null null)\<cdot>(da_h SenderAutomaton (SenderState Sf var_buffer var_c))
          = spfConcOut (tsynbNull (\<C> ''ds''))\<cdot>(da_h SenderAutomaton (SenderState Sf var_buffer var_c))"
   oops
 
-(* Line 42 in the MAA model *)
-lemma tbd_3_2:
+(* Line 42:  Sf -> Sf [buffer.size()>0 && c=0] {as==null, i==null} / {c=3, ds=new Pair<>(buffer.last(),false)}; *)
+lemma step_3_2:
   assumes "(size var_buffer)>0 \<and> var_c=0"
-    shows "spfConcIn  (tsynbNull (\<C> ''as'') \<uplus> tsynbNull (\<C> ''i''))\<cdot>(da_h SenderAutomaton (SenderState Sf var_buffer var_c))
+    shows "spfConcIn  (createBundle_As_I null null)\<cdot>(da_h SenderAutomaton (SenderState Sf var_buffer var_c))
          = spfConcOut (sbe2SB (createDsBundle (Pair (last var_buffer) False)))\<cdot>(da_h SenderAutomaton (SenderState Sf var_buffer 3))"
   oops
 
-(* Line 25 in the MAA model *)
-lemma tbd_4_0:
+(* Line 25:  St -> St [buffer.size()=0 && as!=null && i!=null] / {buffer=buffer.prepend(i), c=3, ds=new Pair<>(i,true)}; *)
+lemma step_4_0:
   assumes "(size var_buffer)=0"
-    shows "spfConcIn  (sbe2SB (createAsBundle port_as) \<uplus> sbe2SB (createIBundle port_i))\<cdot>(da_h SenderAutomaton (SenderState St var_buffer var_c))
+    shows "spfConcIn  (createBundle_As_I (Msg port_as) (Msg port_i))\<cdot>(da_h SenderAutomaton (SenderState St var_buffer var_c))
          = spfConcOut (sbe2SB (createDsBundle (Pair port_i True)))\<cdot>(da_h SenderAutomaton (SenderState St (prepend var_buffer port_i) 3))"
   oops
 
-(* Line 27 in the MAA model *)
-lemma tbd_4_1:
+(* Line 27:  St -> Sf [buffer.size()>1 && i!=null] {as==true} / {buffer=buffer.butlast().prepend(i), c=3, ds=new Pair<>(buffer.butlast().last(),false)}; *)
+lemma step_4_1:
   assumes "(size var_buffer)>1 \<and> port_as=True"
-    shows "spfConcIn  (sbe2DB (createAsBundle port_as) \<uplus> sbe2SB (createIBundle port_i))\<cdot>(da_h SenderAutomaton (SenderState St var_buffer var_c))
+    shows "spfConcIn  (createBundle_As_I (Msg port_as) (Msg port_i))\<cdot>(da_h SenderAutomaton (SenderState St var_buffer var_c))
          = spfConcOut (sbe2SB (createDsBundle (Pair (last (butlast var_buffer)) False)))\<cdot>(da_h SenderAutomaton (SenderState Sf (prepend (butlast var_buffer) port_i) 3))"
   oops
 
-(* Line 28 in the MAA model *)
-lemma tbd_4_2:
+(* Line 28:  St -> St [buffer.size()>0 && c>0 && i!=null] {as==false} / {buffer=buffer.prepend(i), c=c-1}; *)
+lemma step_4_2:
   assumes "(size var_buffer)>0 \<and> var_c>0 \<and> port_as=False"
-    shows "spfConcIn  (sbe2DB (createAsBundle port_as) \<uplus> sbe2SB (createIBundle port_i))\<cdot>(da_h SenderAutomaton (SenderState St var_buffer var_c))
+    shows "spfConcIn  (createBundle_As_I (Msg port_as) (Msg port_i))\<cdot>(da_h SenderAutomaton (SenderState St var_buffer var_c))
          = spfConcOut (tsynbNull (\<C> ''ds''))\<cdot>(da_h SenderAutomaton (SenderState St (prepend var_buffer port_i) (var_c-1)))"
   oops
 
-(* Line 30 in the MAA model *)
-lemma tbd_4_3:
+(* Line 30:  St -> St [buffer.size()>0 && c=0 && i!=null] {as==false} / {buffer=buffer.prepend(i), c=3, ds=new Pair<>(buffer.last(),true)}; *)
+lemma step_4_3:
   assumes "(size var_buffer)>0 \<and> var_c=0 \<and> port_as=False"
-    shows "spfConcIn  (sbe2DB (createAsBundle port_as) \<uplus> sbe2SB (createIBundle port_i))\<cdot>(da_h SenderAutomaton (SenderState St var_buffer var_c))
+    shows "spfConcIn  (createBundle_As_I (Msg port_as) (Msg port_i))\<cdot>(da_h SenderAutomaton (SenderState St var_buffer var_c))
          = spfConcOut (sbe2SB (createDsBundle (Pair (last var_buffer) True)))\<cdot>(da_h SenderAutomaton (SenderState St (prepend var_buffer port_i) 3))"
   oops
 
-(* Line 32 in the MAA model *)
-lemma tbd_4_4:
+(* Line 32:  St -> Sf [buffer.size()=1 && i!=null] {as==true} / {buffer=buffer.butlast().prepend(i), c=3, ds=new Pair<>(i,false)}; *)
+lemma step_4_4:
   assumes "(size var_buffer)=1 \<and> port_as=True"
-    shows "spfConcIn  (sbe2DB (createAsBundle port_as) \<uplus> sbe2SB (createIBundle port_i))\<cdot>(da_h SenderAutomaton (SenderState St var_buffer var_c))
+    shows "spfConcIn  (createBundle_As_I (Msg port_as) (Msg port_i))\<cdot>(da_h SenderAutomaton (SenderState St var_buffer var_c))
          = spfConcOut (sbe2SB (createDsBundle (Pair port_i False)))\<cdot>(da_h SenderAutomaton (SenderState Sf (prepend (butlast var_buffer) port_i) 3))"
   oops
 
-(* Line 17 in the MAA model *)
-lemma tbd_5_0:
+(* Line 17:  St -> St [buffer.size()=0 && as!=null] {i==null}; *)
+lemma step_5_0:
   assumes "(size var_buffer)=0"
-    shows "spfConcIn  (sbe2SB (createAsBundle port_as) \<uplus> tsynbNull (\<C> ''i''))\<cdot>(da_h SenderAutomaton (SenderState St var_buffer var_c))
+    shows "spfConcIn  (createBundle_As_I (Msg port_as) null)\<cdot>(da_h SenderAutomaton (SenderState St var_buffer var_c))
          = spfConcOut (tsynbNull (\<C> ''ds''))\<cdot>(da_h SenderAutomaton (SenderState St var_buffer var_c))"
   oops
 
-(* Line 18 in the MAA model *)
-lemma tbd_5_1:
+(* Line 18:  St -> Sf [buffer.size()>1] {as==true, i==null} / {buffer=buffer.butlast(), c=3, ds=new Pair<>(buffer.butlast().last(),false)}; *)
+lemma step_5_1:
   assumes "(size var_buffer)>1 \<and> port_as=True"
-    shows "spfConcIn  (sbe2DB (createAsBundle port_as) \<uplus> tsynbNull (\<C> ''i''))\<cdot>(da_h SenderAutomaton (SenderState St var_buffer var_c))
+    shows "spfConcIn  (createBundle_As_I (Msg port_as) null)\<cdot>(da_h SenderAutomaton (SenderState St var_buffer var_c))
          = spfConcOut (sbe2SB (createDsBundle (Pair (last (butlast var_buffer)) False)))\<cdot>(da_h SenderAutomaton (SenderState Sf (butlast var_buffer) 3))"
   oops
 
-(* Line 20 in the MAA model *)
-lemma tbd_5_2:
+(* Line 20:  St -> St [buffer.size()>0 && c>0] {as==false, i==null} / {c=c-1}; *)
+lemma step_5_2:
   assumes "(size var_buffer)>0 \<and> var_c>0 \<and> port_as=False"
-    shows "spfConcIn  (sbe2DB (createAsBundle port_as) \<uplus> tsynbNull (\<C> ''i''))\<cdot>(da_h SenderAutomaton (SenderState St var_buffer var_c))
+    shows "spfConcIn  (createBundle_As_I (Msg port_as) null)\<cdot>(da_h SenderAutomaton (SenderState St var_buffer var_c))
          = spfConcOut (tsynbNull (\<C> ''ds''))\<cdot>(da_h SenderAutomaton (SenderState St var_buffer (var_c-1)))"
   oops
 
-(* Line 22 in the MAA model *)
-lemma tbd_5_3:
+(* Line 22:  St -> St [buffer.size()>0 && c=0] {as==false, i==null} / {c=3, ds=new Pair<>(buffer.last(),true)}; *)
+lemma step_5_3:
   assumes "(size var_buffer)>0 \<and> var_c=0 \<and> port_as=False"
-    shows "spfConcIn  (sbe2DB (createAsBundle port_as) \<uplus> tsynbNull (\<C> ''i''))\<cdot>(da_h SenderAutomaton (SenderState St var_buffer var_c))
+    shows "spfConcIn  (createBundle_As_I (Msg port_as) null)\<cdot>(da_h SenderAutomaton (SenderState St var_buffer var_c))
          = spfConcOut (sbe2SB (createDsBundle (Pair (last var_buffer) True)))\<cdot>(da_h SenderAutomaton (SenderState St var_buffer 3))"
   oops
 
-(* Line 24 in the MAA model *)
-lemma tbd_5_4:
+(* Line 24:  St -> Sf [buffer.size()=1] {as==true, i==null} / {buffer=buffer.butlast()}; *)
+lemma step_5_4:
   assumes "(size var_buffer)=1 \<and> port_as=True"
-    shows "spfConcIn  (sbe2DB (createAsBundle port_as) \<uplus> tsynbNull (\<C> ''i''))\<cdot>(da_h SenderAutomaton (SenderState St var_buffer var_c))
+    shows "spfConcIn  (createBundle_As_I (Msg port_as) null)\<cdot>(da_h SenderAutomaton (SenderState St var_buffer var_c))
          = spfConcOut (tsynbNull (\<C> ''ds''))\<cdot>(da_h SenderAutomaton (SenderState Sf (butlast var_buffer) var_c))"
   oops
 
-(* Line 26 in the MAA model *)
-lemma tbd_6_0:
+(* Line 26:  St -> St [buffer.size()=0 && i!=null] {as==null} / {buffer=buffer.prepend(i), c=3, ds=new Pair<>(i,true)}; *)
+lemma step_6_0:
   assumes "(size var_buffer)=0"
-    shows "spfConcIn  (tsynbNull (\<C> ''as'') \<uplus> sbe2SB (createIBundle port_i))\<cdot>(da_h SenderAutomaton (SenderState St var_buffer var_c))
+    shows "spfConcIn  (createBundle_As_I null (Msg port_i))\<cdot>(da_h SenderAutomaton (SenderState St var_buffer var_c))
          = spfConcOut (sbe2SB (createDsBundle (Pair port_i True)))\<cdot>(da_h SenderAutomaton (SenderState St (prepend var_buffer port_i) 3))"
   oops
 
-(* Line 29 in the MAA model *)
-lemma tbd_6_1:
+(* Line 29:  St -> St [buffer.size()>0 && c>0 && i!=null] {as==null} / {buffer=buffer.prepend(i), c=c-1}; *)
+lemma step_6_1:
   assumes "(size var_buffer)>0 \<and> var_c>0"
-    shows "spfConcIn  (tsynbNull (\<C> ''as'') \<uplus> sbe2SB (createIBundle port_i))\<cdot>(da_h SenderAutomaton (SenderState St var_buffer var_c))
+    shows "spfConcIn  (createBundle_As_I null (Msg port_i))\<cdot>(da_h SenderAutomaton (SenderState St var_buffer var_c))
          = spfConcOut (tsynbNull (\<C> ''ds''))\<cdot>(da_h SenderAutomaton (SenderState St (prepend var_buffer port_i) (var_c-1)))"
   oops
 
-(* Line 31 in the MAA model *)
-lemma tbd_6_2:
+(* Line 31:  St -> St [buffer.size()>0 && c=0 && i!=null] {as==null} / {buffer=buffer.prepend(i), c=3, ds=new Pair<>(buffer.last(),true)}; *)
+lemma step_6_2:
   assumes "(size var_buffer)>0 \<and> var_c=0"
-    shows "spfConcIn  (tsynbNull (\<C> ''as'') \<uplus> sbe2SB (createIBundle port_i))\<cdot>(da_h SenderAutomaton (SenderState St var_buffer var_c))
+    shows "spfConcIn  (createBundle_As_I null (Msg port_i))\<cdot>(da_h SenderAutomaton (SenderState St var_buffer var_c))
          = spfConcOut (sbe2SB (createDsBundle (Pair (last var_buffer) True)))\<cdot>(da_h SenderAutomaton (SenderState St (prepend var_buffer port_i) 3))"
   oops
 
-(* Line 19 in the MAA model *)
-lemma tbd_7_0:
+(* Line 19:  St -> St [buffer.size()=0] {as==null, i==null}; *)
+lemma step_7_0:
   assumes "(size var_buffer)=0"
-    shows "spfConcIn  (tsynbNull (\<C> ''as'') \<uplus> tsynbNull (\<C> ''i''))\<cdot>(da_h SenderAutomaton (SenderState St var_buffer var_c))
+    shows "spfConcIn  (createBundle_As_I null null)\<cdot>(da_h SenderAutomaton (SenderState St var_buffer var_c))
          = spfConcOut (tsynbNull (\<C> ''ds''))\<cdot>(da_h SenderAutomaton (SenderState St var_buffer var_c))"
   oops
 
-(* Line 21 in the MAA model *)
-lemma tbd_7_1:
+(* Line 21:  St -> St [buffer.size()>0 && c>0] {as==null, i==null} / {c=c-1}; *)
+lemma step_7_1:
   assumes "(size var_buffer)>0 \<and> var_c>0"
-    shows "spfConcIn  (tsynbNull (\<C> ''as'') \<uplus> tsynbNull (\<C> ''i''))\<cdot>(da_h SenderAutomaton (SenderState St var_buffer var_c))
+    shows "spfConcIn  (createBundle_As_I null null)\<cdot>(da_h SenderAutomaton (SenderState St var_buffer var_c))
          = spfConcOut (tsynbNull (\<C> ''ds''))\<cdot>(da_h SenderAutomaton (SenderState St var_buffer (var_c-1)))"
   oops
 
-(* Line 23 in the MAA model *)
-lemma tbd_7_2:
+(* Line 23:  St -> St [buffer.size()>0 && c=0] {as==null, i==null} / {c=3, ds=new Pair<>(buffer.last(),true)}; *)
+lemma step_7_2:
   assumes "(size var_buffer)>0 \<and> var_c=0"
-    shows "spfConcIn  (tsynbNull (\<C> ''as'') \<uplus> tsynbNull (\<C> ''i''))\<cdot>(da_h SenderAutomaton (SenderState St var_buffer var_c))
+    shows "spfConcIn  (createBundle_As_I null null)\<cdot>(da_h SenderAutomaton (SenderState St var_buffer var_c))
          = spfConcOut (sbe2SB (createDsBundle (Pair (last var_buffer) True)))\<cdot>(da_h SenderAutomaton (SenderState St var_buffer 3))"
   oops
 
